feat: AwsKmsMrkAwareSymmetricKeyring (#383)

src/KMS/KMSUtils.dfy
@@ -6,6 +6,7 @@ include "../SDK/EncryptionContext.dfy"
 include "../StandardLibrary/StandardLibrary.dfy"
 include "../StandardLibrary/UInt.dfy"
 include "../Util/UTF8.dfy"
+include "AwsKmsArnParsing.dfy"
 
 module {:extern "KMSUtils"} KMSUtils {
   import EncryptionContext
@@ -13,327 +14,159 @@ module {:extern "KMSUtils"} KMSUtils {
   import opened StandardLibrary
   import opened Wrappers
   import opened UInt = StandardLibrary.UInt
+  import opened AwsKmsArnParsing
   import UTF8
 
   const MAX_GRANT_TOKENS := 10
 
-  type CustomerMasterKey = s: string | ValidFormatCMK(s)
-    witness (ValidCMKAliasFromSuffix("ExampleAlias"); "alias/ExampleAlias")
-
-  predicate method ValidFormatCMK(cmk: string) {
-    ValidFormatCMKKeyARN(cmk) || ValidFormatCMKAlias(cmk) || ValidFormatCMKAliasARN(cmk)
-  }
-
-  predicate method ValidFormatCMKKeyARN(cmk: string) {
-    var components := Split(cmk, ':');
-    UTF8.IsASCIIString(cmk) && 0 < |cmk| <= 2048 && |components| == 6 && components[0] == "arn" && components[2] == "kms" && Split(components[5], '/')[0] == "key"
-  }
-
-  predicate method ValidFormatCMKAlias(cmk: string) {
-    var components := Split(cmk, '/');
-    UTF8.IsASCIIString(cmk) && 0 < |cmk| <= 2048 && |components| == 2 && components[0] == "alias"
-  }
-
-  lemma ValidCMKAliasFromSuffix(suffix: string)
-    requires UTF8.IsASCIIString(suffix) && |suffix| < 2042 && '/' !in suffix
-    ensures var cmk := "alias/" + suffix;
-      ValidFormatCMKAlias(cmk)
-  {
-    var alias := "alias";
-    assert UTF8.IsASCIIString(alias);
-    var cmk := alias + "/" + suffix;
-    assert UTF8.IsASCIIString(cmk);
-
-    var components := Split(cmk, '/');
-    calc {
-      components;
-    ==
-      Split(alias + "/" + suffix, '/');
-    ==  { WillSplitOnDelim(cmk, '/', alias); }
-      [alias] + Split(cmk[|alias| + 1..], '/');
-    ==  { assert cmk[|alias| + 1..] == suffix; }
-      [alias] + Split(suffix, '/');
-    ==  { WillNotSplitWithOutDelim(suffix, '/'); }
-      [alias] + [suffix];
-    ==
-      [alias, suffix];
-    }
-  }
-
-  predicate method ValidFormatCMKAliasARN(cmk: string) {
-    var components := Split(cmk, ':');
-    UTF8.IsASCIIString(cmk) && 0 < |cmk| <= 2048 && |components| == 6 && components[0] == "arn" && components[2] == "kms" && Split(components[5], '/')[0] == "alias"
-  }
-
-  type GrantToken = s: string | 0 < |s| <= 8192 witness "witness"
+  type CustomerMasterKey = AwsKmsIdentifierString
+  type GrantTokens = s: seq<GrantToken> | 0 <= |s| <= MAX_GRANT_TOKENS
+  type GrantToken = s: string | 0 < |s| <= 8192 witness *
 
   datatype ResponseMetadata = ResponseMetadata(metadata: map<string, string>, requestID: string)
 
   type HttpStatusCode = int //FIXME: Restrict this
 
-  datatype GenerateDataKeyRequest = GenerateDataKeyRequest(encryptionContext: EncryptionContext.Map, grantTokens: seq<GrantToken>, keyID: CustomerMasterKey, numberOfBytes: int32)
+  datatype GenerateDataKeyRequest = GenerateDataKeyRequest(
+    encryptionContext: EncryptionContext.Map,
+    grantTokens: seq<GrantToken>,
+    keyID: AwsKmsIdentifierString,
+    numberOfBytes: int32
+  )
   {
     predicate Valid() {
       0 <= |grantTokens| <= MAX_GRANT_TOKENS && 0 < numberOfBytes <= 1024
     }
   }
 
-  datatype GenerateDataKeyResponse = GenerateDataKeyResponse(ciphertextBlob: seq<uint8>, contentLength: int, httpStatusCode: HttpStatusCode, keyID: string, plaintext: seq<uint8>, responseMetadata: ResponseMetadata)
+  datatype GenerateDataKeyResponse = GenerateDataKeyResponse(
+    ciphertextBlob: seq<uint8>,
+    keyID: string,
+    plaintext: seq<uint8>
+  )
   {
     predicate method IsWellFormed() {
       |keyID| < UINT16_LIMIT && |ciphertextBlob| < UINT16_LIMIT
     }
   }
 
-  datatype EncryptRequest = EncryptRequest(encryptionContext: EncryptionContext.Map, grantTokens: seq<GrantToken>, keyID: CustomerMasterKey, plaintext: seq<uint8>)
+  datatype EncryptRequest = EncryptRequest(
+    encryptionContext: EncryptionContext.Map,
+    grantTokens: seq<GrantToken>,
+    keyID: AwsKmsIdentifierString,
+    plaintext: seq<uint8>
+  )
   {
     predicate Valid() {
       0 <= |grantTokens| <= MAX_GRANT_TOKENS
     }
   }
 
-  datatype EncryptResponse = EncryptResponse(ciphertextBlob: seq<uint8>, contentLength: int, httpStatusCode: HttpStatusCode, keyID: string, responseMetadata: ResponseMetadata)
+  datatype EncryptResponse = EncryptResponse(
+    ciphertextBlob: seq<uint8>,
+    contentLength: int,
+    httpStatusCode: HttpStatusCode,
+    keyID: string,
+    responseMetadata: ResponseMetadata
+  )
   {
     predicate method IsWellFormed() {
       |keyID| < UINT16_LIMIT && |ciphertextBlob| < UINT16_LIMIT
     }
   }
 
-  datatype DecryptRequest = DecryptRequest(ciphertextBlob: seq<uint8>, encryptionContext: EncryptionContext.Map, grantTokens: seq<GrantToken>)
+  datatype DecryptRequest = DecryptRequest(
+    keyId: string,
+    ciphertextBlob: seq<uint8>,
+    encryptionContext: EncryptionContext.Map,
+    grantTokens: seq<GrantToken>)
   {
     predicate Valid() {
       0 <= |grantTokens| <= MAX_GRANT_TOKENS
     }
   }
 
-  datatype DecryptResponse = DecryptResponse(contentLength: int, httpStatusCode: HttpStatusCode, keyID: string, plaintext: seq<uint8>, responseMetadata: ResponseMetadata)
+  datatype DecryptResponse = DecryptResponse(
+    contentLength: int,
+    httpStatusCode: HttpStatusCode,
+    keyID: string,
+    plaintext: seq<uint8>,
+    responseMetadata: ResponseMetadata
+  )
 
   method {:extern "KMSUtils.ClientHelper", "GetDefaultAWSKMSServiceClientExtern"} GetDefaultAWSKMSServiceClientExtern(region: Option<string>) returns (res: Result<IAmazonKeyManagementService, string>)
 
-  method {:extern "KMSUtils.ClientHelper", "GenerateDataKey"} GenerateDataKey(client: IAmazonKeyManagementService, request: GenerateDataKeyRequest) returns (res: Result<GenerateDataKeyResponse, string>)
-    requires request.Valid()
+// The {:opaque} is important. 
+// These predicates are hacks to model the fact that a particular external method was called for the verifier,
+// but depends on the post-condition of the method being the ONLY way to prove the predicate is true for any particular arguments. 
+// Making the predicate opaque means that other code cannot prove them true,
+// UNLESS the other code reveals them.
+  predicate {:opaque} GenerateDataKeyCalledWith(
+    client: IAmazonKeyManagementService,
+    request: GenerateDataKeyRequest
+  ) {true}
+  predicate {:opaque} GenerateDataKeyResult(
+    ciphertextBlob: seq<uint8>,
+    plaintext: seq<uint8>
+  ) {true}
 
-  method {:extern "KMSUtils.ClientHelper", "Encrypt"} Encrypt(client: IAmazonKeyManagementService, request: EncryptRequest) returns (res: Result<EncryptResponse, string>)
-    requires request.Valid()
+  predicate {:opaque} EncryptCalledWith(
+    client: IAmazonKeyManagementService,
+    request: EncryptRequest
+  ) {true}
+  predicate {:opaque} EncryptResult(
+    ciphertextBlob: seq<uint8>
+  ) {true}
 
-  method {:extern "KMSUtils.ClientHelper", "Decrypt"} Decrypt(client: IAmazonKeyManagementService, request: DecryptRequest) returns (res: Result<DecryptResponse, string>)
-    requires request.Valid()
+  predicate {:opaque} DecryptCalledWith(
+    client: IAmazonKeyManagementService,
+    request: DecryptRequest
+  ) {true}
+  predicate {:opaque} DecryptResult(
+    keyID: string,
+    plaintext: seq<uint8>
+  ) {true}
 
-  method {:extern "KMSUtils.ClientHelper", "AddCachingClientCallback"} AddCachingClientCallback(client: IAmazonKeyManagementService, region: Option<string>, cache: CachingClientSupplierCache)
+  method {:extern "KMSUtils.ClientHelper", "GenerateDataKey"} GenerateDataKey(
+    client: IAmazonKeyManagementService,
+    request: GenerateDataKeyRequest
+  ) 
+    returns (res: Result<GenerateDataKeyResponse, string>)
+    requires request.Valid()
+    ensures GenerateDataKeyCalledWith(client, request)
+    ensures res.Success? ==>
+      var r := res.value;
+      GenerateDataKeyResult(r.ciphertextBlob, r.plaintext)
+
+  method {:extern "KMSUtils.ClientHelper", "Encrypt"} Encrypt(
+    client: IAmazonKeyManagementService,
+    request: EncryptRequest
+  )
+    returns (res: Result<EncryptResponse, string>)
+    requires request.Valid()
+    ensures EncryptCalledWith(client, request)
+    ensures res.Success? ==> EncryptResult(res.value.ciphertextBlob)
+
+  method {:extern "KMSUtils.ClientHelper", "Decrypt"} Decrypt(
+    client: IAmazonKeyManagementService,
+    request: DecryptRequest
+  ) returns (res: Result<DecryptResponse, string>)
+    requires request.Valid()
+    ensures DecryptCalledWith(client, request)
+    ensures res.Success? ==>
+      var r := res.value;
+      DecryptResult(r.keyID, r.plaintext)
 
   trait {:extern "DafnyAWSKMSClientSupplier"} DafnyAWSKMSClientSupplier {
-    ghost var Repr: set<object>
-
-    predicate Valid()
-      reads this, Repr
-      ensures Valid() ==> this in Repr
-
     method GetClient(region: Option<string>) returns (res: Result<IAmazonKeyManagementService, string>)
-      requires Valid()
-      ensures Valid()
-      decreases Repr
-  }
-
-  // An implementation of a DafnyAWSKMSClientSupplier that takes in an existing DafnyAWSKMSClientSupplier as well as a seq of regions (strings).
-  // The LimitRegionsClientSupplier will only return an AWS KMS service client from the given DafnyAWSKMSClientSupplier
-  // if the region provided to GetClient(region) is in the list of regions associated with the LimitRegionsClientSupplier.
-  class LimitRegionsClientSupplier extends DafnyAWSKMSClientSupplier {
-    const clientSupplier: DafnyAWSKMSClientSupplier
-    const regions: seq<string>
-
-    predicate Valid()
-      reads this, Repr
-      ensures Valid() ==> this in Repr
-    {
-      this in Repr &&
-      clientSupplier in Repr && clientSupplier.Repr <= Repr && this !in clientSupplier.Repr && clientSupplier.Valid()
-    }
-
-    constructor(clientSupplier: DafnyAWSKMSClientSupplier, regions: seq<string>)
-      requires clientSupplier.Valid()
-      ensures this.clientSupplier == clientSupplier
-      ensures this.regions == regions
-      ensures Valid() && fresh(Repr - clientSupplier.Repr)
-    {
-      this.clientSupplier := clientSupplier;
-      this.regions := regions;
-      Repr := {this} + clientSupplier.Repr;
-    }
-
-    method GetClient(region: Option<string>) returns (res: Result<IAmazonKeyManagementService, string>)
-      requires Valid()
-      ensures Valid()
-      // Verify this behavior with the spec. TODO: https://github.com/awslabs/aws-encryption-sdk-dafny/issues/272
-      // Only add a post condition around failures, since the GetClient call could return a success or failure
-      ensures region.None? ==> res.Failure?
-      ensures region.Some? && !(region.value in regions) ==> res.Failure?
-      decreases Repr
-    {
-      // In order to limit regions, make sure our given region string exists and is a member of the regions to limit to
-      if region.Some? && region.value in regions {
-        var resClient := clientSupplier.GetClient(region);
-        return resClient;
-      } else if region.None? {
-        return Result.Failure("LimitRegionsClientSupplier GetClient requires a region");
-      }
-      var failure := "Given region " + region.value + " not in regions maintained by LimitRegionsClientSupplier";
-      return Result.Failure(failure);
-    }
-  }
-
-  // An implementation of a DafnyAWSKMSClientSupplier that takes in an existing DafnyAWSKMSClientSupplier as well as a seq of regions (strings).
-  // The ExcludeRegionsClientSupplier will only return an AWS KMS service client from the given DafnyAWSKMSClientSupplier
-  // if the region provided to GetClient(region) is not in the list of regions associated with the ExcludeRegionsClientSupplier.
-  class ExcludeRegionsClientSupplier extends DafnyAWSKMSClientSupplier {
-    const clientSupplier: DafnyAWSKMSClientSupplier
-    const regions: seq<string>
-
-    predicate Valid()
-      reads this, Repr
-      ensures Valid() ==> this in Repr
-    {
-      this in Repr &&
-      clientSupplier in Repr && clientSupplier.Repr <= Repr && this !in clientSupplier.Repr && clientSupplier.Valid()
-    }
-
-    constructor(clientSupplier: DafnyAWSKMSClientSupplier, regions: seq<string>)
-      requires clientSupplier.Valid()
-      ensures this.clientSupplier == clientSupplier
-      ensures this.regions == regions
-      ensures Valid() && fresh(Repr - clientSupplier.Repr)
-    {
-      this.clientSupplier := clientSupplier;
-      this.regions := regions;
-      Repr := {this} + clientSupplier.Repr;
-    }
-
-    method GetClient(region: Option<string>) returns (res: Result<IAmazonKeyManagementService, string>)
-      requires Valid()
-      ensures Valid()
-      // Verify this behavior with the spec. TODO: https://github.com/awslabs/aws-encryption-sdk-dafny/issues/272
-      // Only add a post condition around failures, since the GetClient call could return a success or failure
-      ensures region.None? ==> res.Failure?
-      ensures region.Some? && region.value in regions ==> res.Failure?
-      decreases Repr
-    {
-      // In order to exclude regions, make sure our given region string exists and is not a member of the regions to exclude
-      if region.None? {
-        return Result.Failure("ExcludeRegionsClientSupplier GetClient requires a region");
-      } else if (region.Some? && region.value in regions) {
-        var failure := "Given region " + region.value + " is in regions maintained by ExcludeRegionsClientSupplier";
-        return Result.Failure(failure);
-      }
-      var resClient := clientSupplier.GetClient(region);
-      return resClient;
-    }
-  }
-
-  class CachingClientSupplierCache {
-    ghost var Repr: set<object>
-    var ClientCache: map<Option<string>, IAmazonKeyManagementService>
-
-    predicate Valid()
-      reads this, Repr
-      ensures Valid() ==> this in Repr
-    {
-      this in Repr &&
-      (forall region :: region in ClientCache.Keys ==> ClientCache[region] in Repr)
-    }
-
-    constructor ()
-      ensures ClientCache == map[]
-      ensures Valid() && fresh(Repr)
-    {
-      ClientCache := map[];
-      Repr := {this};
-    }
-
-    function method LookupClient(region: Option<string>): (client: Option<IAmazonKeyManagementService>)
-      requires Valid()
-      ensures Valid()
-      ensures client.Some? ==> region in ClientCache.Keys && client.value in Repr
-      reads Repr
-    {
-      if region in ClientCache.Keys then Some(ClientCache[region]) else None()
-    }
-
-    method AddClient(region: Option<string>, client: IAmazonKeyManagementService)
-      requires Valid()
-      ensures Valid()
-      ensures region in ClientCache.Keys && ClientCache[region] == client && client in Repr
-      modifies Repr
-    {
-      Repr := Repr + {client};
-      ClientCache := ClientCache[region := client];
-    }
-  }
-
-  class CachingClientSupplier extends DafnyAWSKMSClientSupplier {
-    const clientSupplier: DafnyAWSKMSClientSupplier
-    const clientCache: CachingClientSupplierCache
-
-    predicate Valid()
-      reads this, Repr
-      ensures Valid() ==> this in Repr
-    {
-      this in Repr &&
-      clientSupplier in Repr && clientSupplier.Repr <= Repr && this !in clientSupplier.Repr && clientSupplier.Valid() &&
-      clientCache in Repr && clientCache.Repr <= Repr && this !in clientCache.Repr && clientCache.Valid() &&
-      clientSupplier.Repr !! clientCache.Repr
-    }
-
-    constructor(clientSupplier: DafnyAWSKMSClientSupplier)
-      requires clientSupplier.Valid()
-      ensures this.clientSupplier == clientSupplier
-      ensures Valid() && fresh(Repr - clientSupplier.Repr)
-    {
-      this.clientSupplier := clientSupplier;
-      // Establish the cache
-      var clientCache := new CachingClientSupplierCache();
-      assert clientCache in clientCache.Repr;
-      this.clientCache := clientCache;
-      Repr := {this} + clientSupplier.Repr + clientCache.Repr;
-    }
-
-    method GetClient(region: Option<string>) returns (res: Result<IAmazonKeyManagementService, string>)
-      requires Valid()
-      ensures Valid()
-      ensures clientCache.LookupClient(region).Some? ==> res.Success? && clientCache.LookupClient(region).value == res.value
-      decreases Repr
-    {
-      var potentialClient := clientCache.LookupClient(region);
-      if potentialClient.Some? {
-        return Result.Success(potentialClient.value);
-      } else  {
-        var resClient := clientSupplier.GetClient(region);
-        if resClient.Success? {
-          // Call the extern method to create a callback for adding the client to the cache
-          AddCachingClientCallback(resClient.value, region, clientCache);
-        }
-        return resClient;
-      }
-    }
   }
 
   class BaseClientSupplier extends DafnyAWSKMSClientSupplier {
-    predicate Valid()
-      reads this, Repr
-      ensures Valid() ==> this in Repr
-    {
-      this in Repr
-    }
 
-    constructor()
-      ensures Valid() && fresh(Repr)
-    {
-      Repr := {this};
-    }
+    constructor(){}
 
     // Since this is the base client supplier, this just calls the extern GetClient method
     method GetClient(region: Option<string>) returns (res: Result<IAmazonKeyManagementService, string>)
-      requires Valid()
-      ensures Valid()
-      decreases Repr
     {
       // Since this is the base client supplier, this obtains the extern client
       var resClient := GetDefaultAWSKMSServiceClientExtern(region);
