src/SDK/Keyring/AwsKms/Constants.dfy
@@ -1,0 +1,14 @@
+// Copyright Amazon.com Inc. or its affiliates. All Rights Reserved.
+// SPDX-License-Identifier: Apache-2.0
+
+include "../../../Util/UTF8.dfy"
+
+module Constants {
+  import UTF8
+
+  // UTF-8 encoded "aws-kms"
+  const PROVIDER_ID: UTF8.ValidUTF8Bytes :=
+    var s := [0x61, 0x77, 0x73, 0x2D, 0x6B, 0x6D, 0x73];
+    assert UTF8.ValidUTF8Range(s, 0, 7);
+    s
+}
