src/SDK/Keyring/KMSKeyring.dfy
@@ -1,222 +1,222 @@
-// Copyright Amazon.com Inc. or its affiliates. All Rights Reserved.
-// SPDX-License-Identifier: Apache-2.0
+// // Copyright Amazon.com Inc. or its affiliates. All Rights Reserved.
+// // SPDX-License-Identifier: Apache-2.0
 
-include "./Defs.dfy"
-include "../Materials.dfy"
-include "../AlgorithmSuite.dfy"
-include "../../StandardLibrary/StandardLibrary.dfy"
-include "../../KMS/KMSUtils.dfy"
-include "../../Util/UTF8.dfy"
+// include "./Defs.dfy"
+// include "../Materials.dfy"
+// include "../AlgorithmSuite.dfy"
+// include "../../StandardLibrary/StandardLibrary.dfy"
+// include "../../KMS/KMSUtils.dfy"
+// include "../../Util/UTF8.dfy"
 
-module {:extern "KMSKeyringDef"} KMSKeyringDef {
-  import opened StandardLibrary
-  import opened Wrappers
-  import opened UInt = StandardLibrary.UInt
-  import AlgorithmSuite
-  import KeyringDefs
-  import Mat = Materials
-  import KMSUtils
-  import UTF8
+// module {:extern "KMSKeyringDef"} KMSKeyringDef {
+//   import opened StandardLibrary
+//   import opened Wrappers
+//   import opened UInt = StandardLibrary.UInt
+//   import AlgorithmSuite
+//   import KeyringDefs
+//   import Mat = Materials
+//   import KMSUtils
+//   import UTF8
 
-  // UTF-8 encoded "aws-kms"
-  const PROVIDER_ID: UTF8.ValidUTF8Bytes :=
-    var s := [0x61, 0x77, 0x73, 0x2D, 0x6B, 0x6D, 0x73];
-    assert UTF8.ValidUTF8Range(s, 0, 7);
-    s
+//   // UTF-8 encoded "aws-kms"
+//   const PROVIDER_ID: UTF8.ValidUTF8Bytes :=
+//     var s := [0x61, 0x77, 0x73, 0x2D, 0x6B, 0x6D, 0x73];
+//     assert UTF8.ValidUTF8Range(s, 0, 7);
+//     s
 
-  function method RegionFromKMSKeyARN(arn: KMSUtils.CustomerMasterKey): Result<string, string>
-  {
-    var components := Split(arn, ':');
-    if 6 <= |components| && components[0] == "arn" && components[2] == "kms" then Success(components[3]) else Failure("Malformed ARN")
-  }
+//   function method RegionFromKMSKeyARN(arn: KMSUtils.CustomerMasterKey): Result<string, string>
+//   {
+//     var components := Split(arn, ':');
+//     if 6 <= |components| && components[0] == "arn" && components[2] == "kms" then Success(components[3]) else Failure("Malformed ARN")
+//   }
 
-  class KMSKeyring extends KeyringDefs.Keyring {
+//   class KMSKeyring extends KeyringDefs.Keyring {
 
-    const clientSupplier: KMSUtils.DafnyAWSKMSClientSupplier
-    const keyIDs: seq<KMSUtils.CustomerMasterKey>
-    const generator: Option<KMSUtils.CustomerMasterKey>
-    const grantTokens: seq<KMSUtils.GrantToken>
-    const isDiscovery: bool
+//     const clientSupplier: KMSUtils.DafnyAWSKMSClientSupplier
+//     const keyIDs: seq<KMSUtils.CustomerMasterKey>
+//     const generator: Option<KMSUtils.CustomerMasterKey>
+//     const grantTokens: seq<KMSUtils.GrantToken>
+//     const isDiscovery: bool
 
-    predicate Valid()
-      reads this, Repr
-      ensures Valid() ==> this in Repr
-    {
-      && this in Repr
-      && 0 <= |grantTokens| <= KMSUtils.MAX_GRANT_TOKENS
-      && (|keyIDs| == 0 && generator.None? ==> isDiscovery)
-      && (clientSupplier in Repr && clientSupplier.Repr <= Repr && this !in clientSupplier.Repr && clientSupplier.Valid())
-    }
+//     predicate Valid()
+//       reads this, Repr
+//       ensures Valid() ==> this in Repr
+//     {
+//       && this in Repr
+//       && 0 <= |grantTokens| <= KMSUtils.MAX_GRANT_TOKENS
+//       && (|keyIDs| == 0 && generator.None? ==> isDiscovery)
+//       && (clientSupplier in Repr && clientSupplier.Repr <= Repr && this !in clientSupplier.Repr && clientSupplier.Valid())
+//     }
 
-    constructor (clientSupplier: KMSUtils.DafnyAWSKMSClientSupplier, keyIDs: seq<KMSUtils.CustomerMasterKey>, generator: Option<KMSUtils.CustomerMasterKey>, grantTokens: seq<KMSUtils.GrantToken>)
-      requires clientSupplier.Valid()
-      requires 0 <= |grantTokens| <= KMSUtils.MAX_GRANT_TOKENS
-      ensures this.clientSupplier == clientSupplier
-      ensures Valid() && fresh(Repr - clientSupplier.Repr)
-    {
-      this.clientSupplier := clientSupplier;
-      this.keyIDs         := keyIDs;
-      this.generator      := generator;
-      this.grantTokens    := grantTokens;
+//     constructor (clientSupplier: KMSUtils.DafnyAWSKMSClientSupplier, keyIDs: seq<KMSUtils.CustomerMasterKey>, generator: Option<KMSUtils.CustomerMasterKey>, grantTokens: seq<KMSUtils.GrantToken>)
+//       requires clientSupplier.Valid()
+//       requires 0 <= |grantTokens| <= KMSUtils.MAX_GRANT_TOKENS
+//       ensures this.clientSupplier == clientSupplier
+//       ensures Valid() && fresh(Repr - clientSupplier.Repr)
+//     {
+//       this.clientSupplier := clientSupplier;
+//       this.keyIDs         := keyIDs;
+//       this.generator      := generator;
+//       this.grantTokens    := grantTokens;
 
-      this.isDiscovery    := |keyIDs| == 0 && generator.None?;
-      Repr := {this} + clientSupplier.Repr;
-    }
+//       this.isDiscovery    := |keyIDs| == 0 && generator.None?;
+//       Repr := {this} + clientSupplier.Repr;
+//     }
 
-    method Generate(materials: Mat.ValidEncryptionMaterials) returns (res: Result<Mat.ValidEncryptionMaterials, string>)
-      requires Valid()
-      requires generator.Some?
-      requires materials.plaintextDataKey.None?
-      requires |materials.encryptedDataKeys| == 0
-      requires !isDiscovery
-      ensures Valid()
-      ensures res.Success? ==>
-          && materials.encryptionContext == res.value.encryptionContext
-          && materials.algorithmSuiteID == res.value.algorithmSuiteID
-          && res.value.plaintextDataKey.Some?
-          && materials.encryptedDataKeys <= res.value.encryptedDataKeys
-          && materials.signingKey == res.value.signingKey
-    {
-      var generatorRequest := KMSUtils.GenerateDataKeyRequest(materials.encryptionContext, grantTokens, generator.value, materials.algorithmSuiteID.KDFInputKeyLength() as int32);
-      var regionRes := RegionFromKMSKeyARN(generator.value);
-      var regionOpt := regionRes.ToOption();
-      var client :- clientSupplier.GetClient(regionOpt);
-      var generatorResponse :- KMSUtils.GenerateDataKey(client, generatorRequest);
-      if !generatorResponse.IsWellFormed() {
-        return Failure("Invalid response from KMS GenerateDataKey");
-      }
-      var providerInfo :- UTF8.Encode(generatorResponse.keyID);
-      if UINT16_LIMIT <= |providerInfo| {
-        return Failure("providerInfo exceeds maximum length");
-      }
-      var encryptedDataKey := Mat.EncryptedDataKey(PROVIDER_ID, providerInfo, generatorResponse.ciphertextBlob);
-      var keyID := generatorResponse.keyID;
-      var plaintextDataKey := generatorResponse.plaintext;
+//     method Generate(materials: Mat.ValidEncryptionMaterials) returns (res: Result<Mat.ValidEncryptionMaterials, string>)
+//       requires Valid()
+//       requires generator.Some?
+//       requires materials.plaintextDataKey.None?
+//       requires |materials.encryptedDataKeys| == 0
+//       requires !isDiscovery
+//       ensures Valid()
+//       ensures res.Success? ==>
+//           && materials.encryptionContext == res.value.encryptionContext
+//           && materials.algorithmSuiteID == res.value.algorithmSuiteID
+//           && res.value.plaintextDataKey.Some?
+//           && materials.encryptedDataKeys <= res.value.encryptedDataKeys
+//           && materials.signingKey == res.value.signingKey
+//     {
+//       var generatorRequest := KMSUtils.GenerateDataKeyRequest(materials.encryptionContext, grantTokens, generator.value, materials.algorithmSuiteID.KDFInputKeyLength() as int32);
+//       var regionRes := RegionFromKMSKeyARN(generator.value);
+//       var regionOpt := regionRes.ToOption();
+//       var client :- clientSupplier.GetClient(regionOpt);
+//       var generatorResponse :- KMSUtils.GenerateDataKey(client, generatorRequest);
+//       if !generatorResponse.IsWellFormed() {
+//         return Failure("Invalid response from KMS GenerateDataKey");
+//       }
+//       var providerInfo :- UTF8.Encode(generatorResponse.keyID);
+//       if UINT16_LIMIT <= |providerInfo| {
+//         return Failure("providerInfo exceeds maximum length");
+//       }
+//       var encryptedDataKey := Mat.EncryptedDataKey(PROVIDER_ID, providerInfo, generatorResponse.ciphertextBlob);
+//       var keyID := generatorResponse.keyID;
+//       var plaintextDataKey := generatorResponse.plaintext;
 
-      if !materials.algorithmSuiteID.ValidPlaintextDataKey(plaintextDataKey) {
-        return Failure("Invalid response from KMS GenerateDataKey: Invalid key");
-      }
+//       if !materials.algorithmSuiteID.ValidPlaintextDataKey(plaintextDataKey) {
+//         return Failure("Invalid response from KMS GenerateDataKey: Invalid key");
+//       }
 
-      var encodedGenerator :- UTF8.Encode(generator.value);
-      var newEncryptedDataKeys := [encryptedDataKey];
-      var result := materials.WithKeys(Some(plaintextDataKey), newEncryptedDataKeys);
-      return Success(result);
-    }
+//       var encodedGenerator :- UTF8.Encode(generator.value);
+//       var newEncryptedDataKeys := [encryptedDataKey];
+//       var result := materials.WithKeys(Some(plaintextDataKey), newEncryptedDataKeys);
+//       return Success(result);
+//     }
 
-    method OnEncrypt(materials: Mat.ValidEncryptionMaterials) returns (res: Result<Mat.ValidEncryptionMaterials, string>)
-      requires Valid()
-      ensures Valid()
-      ensures res.Success? ==>
-          && materials.encryptionContext == res.value.encryptionContext
-          && materials.algorithmSuiteID == res.value.algorithmSuiteID
-          && (materials.plaintextDataKey.Some? ==> res.value.plaintextDataKey == materials.plaintextDataKey)
-          && materials.encryptedDataKeys <= res.value.encryptedDataKeys
-          && materials.signingKey == res.value.signingKey
-      ensures isDiscovery ==> res.Success? && res.value == materials
-    {
-      if isDiscovery {
-        return Success(materials);
-      } else if materials.plaintextDataKey.None? && generator.None? {
-        return Failure("No plaintext datakey or generator defined");
-      }
+//     method OnEncrypt(materials: Mat.ValidEncryptionMaterials) returns (res: Result<Mat.ValidEncryptionMaterials, string>)
+//       requires Valid()
+//       ensures Valid()
+//       ensures res.Success? ==>
+//           && materials.encryptionContext == res.value.encryptionContext
+//           && materials.algorithmSuiteID == res.value.algorithmSuiteID
+//           && (materials.plaintextDataKey.Some? ==> res.value.plaintextDataKey == materials.plaintextDataKey)
+//           && materials.encryptedDataKeys <= res.value.encryptedDataKeys
+//           && materials.signingKey == res.value.signingKey
+//       ensures isDiscovery ==> res.Success? && res.value == materials
+//     {
+//       if isDiscovery {
+//         return Success(materials);
+//       } else if materials.plaintextDataKey.None? && generator.None? {
+//         return Failure("No plaintext datakey or generator defined");
+//       }
 
-      var encryptCMKs := keyIDs;
-      var resultMaterials: Mat.ValidEncryptionMaterials;
-      if generator.Some? {
-        if materials.plaintextDataKey.None? {
-          resultMaterials :- Generate(materials);
-          assert resultMaterials.plaintextDataKey.Some?;
-        } else {
-          resultMaterials := materials;
-          encryptCMKs := encryptCMKs + [generator.value];
-        }
-      } else {
-        resultMaterials := materials;
-      }
-      assert resultMaterials.plaintextDataKey.Some?;
-      assert materials.plaintextDataKey.Some? ==> resultMaterials.plaintextDataKey == materials.plaintextDataKey;
+//       var encryptCMKs := keyIDs;
+//       var resultMaterials: Mat.ValidEncryptionMaterials;
+//       if generator.Some? {
+//         if materials.plaintextDataKey.None? {
+//           resultMaterials :- Generate(materials);
+//           assert resultMaterials.plaintextDataKey.Some?;
+//         } else {
+//           resultMaterials := materials;
+//           encryptCMKs := encryptCMKs + [generator.value];
+//         }
+//       } else {
+//         resultMaterials := materials;
+//       }
+//       assert resultMaterials.plaintextDataKey.Some?;
+//       assert materials.plaintextDataKey.Some? ==> resultMaterials.plaintextDataKey == materials.plaintextDataKey;
 
-      var i := 0;
-      while i < |encryptCMKs|
-          invariant resultMaterials.plaintextDataKey.Some?
-          invariant materials.encryptionContext == resultMaterials.encryptionContext
-          invariant materials.algorithmSuiteID == resultMaterials.algorithmSuiteID
-          invariant materials.plaintextDataKey.Some? ==> resultMaterials.plaintextDataKey == materials.plaintextDataKey
-          invariant materials.encryptedDataKeys <= resultMaterials.encryptedDataKeys
-          invariant materials.signingKey == resultMaterials.signingKey
-      {
-        var encryptRequest := KMSUtils.EncryptRequest(materials.encryptionContext, grantTokens, encryptCMKs[i], resultMaterials.plaintextDataKey.value);
-        var regionRes := RegionFromKMSKeyARN(encryptCMKs[i]);
-        var regionOpt := regionRes.ToOption();
-        var client :- clientSupplier.GetClient(regionOpt);
-        var encryptResponse :- KMSUtils.Encrypt(client, encryptRequest);
-        if encryptResponse.IsWellFormed() {
-          var providerInfo :- UTF8.Encode(encryptResponse.keyID);
-          if UINT16_LIMIT <= |providerInfo| {
-            return Failure("providerInfo exceeds maximum length");
-          }
-          var edk := Mat.EncryptedDataKey(PROVIDER_ID, providerInfo, encryptResponse.ciphertextBlob);
-          var encodedEncryptCMK :- UTF8.Encode(encryptCMKs[i]);
-          resultMaterials := resultMaterials.WithKeys(resultMaterials.plaintextDataKey, [edk]);
-        } else {
-          return Failure("Invalid response from KMS Encrypt");
-        }
-        i := i + 1;
-      }
-      return Success(resultMaterials);
-    }
+//       var i := 0;
+//       while i < |encryptCMKs|
+//           invariant resultMaterials.plaintextDataKey.Some?
+//           invariant materials.encryptionContext == resultMaterials.encryptionContext
+//           invariant materials.algorithmSuiteID == resultMaterials.algorithmSuiteID
+//           invariant materials.plaintextDataKey.Some? ==> resultMaterials.plaintextDataKey == materials.plaintextDataKey
+//           invariant materials.encryptedDataKeys <= resultMaterials.encryptedDataKeys
+//           invariant materials.signingKey == resultMaterials.signingKey
+//       {
+//         var encryptRequest := KMSUtils.EncryptRequest(materials.encryptionContext, grantTokens, encryptCMKs[i], resultMaterials.plaintextDataKey.value);
+//         var regionRes := RegionFromKMSKeyARN(encryptCMKs[i]);
+//         var regionOpt := regionRes.ToOption();
+//         var client :- clientSupplier.GetClient(regionOpt);
+//         var encryptResponse :- KMSUtils.Encrypt(client, encryptRequest);
+//         if encryptResponse.IsWellFormed() {
+//           var providerInfo :- UTF8.Encode(encryptResponse.keyID);
+//           if UINT16_LIMIT <= |providerInfo| {
+//             return Failure("providerInfo exceeds maximum length");
+//           }
+//           var edk := Mat.EncryptedDataKey(PROVIDER_ID, providerInfo, encryptResponse.ciphertextBlob);
+//           var encodedEncryptCMK :- UTF8.Encode(encryptCMKs[i]);
+//           resultMaterials := resultMaterials.WithKeys(resultMaterials.plaintextDataKey, [edk]);
+//         } else {
+//           return Failure("Invalid response from KMS Encrypt");
+//         }
+//         i := i + 1;
+//       }
+//       return Success(resultMaterials);
+//     }
 
-    predicate method ShouldAttemptDecryption(providerInfo: string)
-    {
-      var keys := if generator.Some? then keyIDs + [generator.value] else keyIDs;
-      KMSUtils.ValidFormatCMK(providerInfo)
-        && (isDiscovery || providerInfo in keys)
-    }
+//     predicate method ShouldAttemptDecryption(providerInfo: string)
+//     {
+//       var keys := if generator.Some? then keyIDs + [generator.value] else keyIDs;
+//       KMSUtils.ValidFormatCMK(providerInfo)
+//         && (isDiscovery || providerInfo in keys)
+//     }
 
-    method OnDecrypt(materials: Mat.ValidDecryptionMaterials, edks: seq<Mat.EncryptedDataKey>) returns (res: Result<Mat.ValidDecryptionMaterials, string>)
-      requires Valid()
-      ensures Valid()
-      ensures |edks| == 0 ==> res.Success? && materials == res.value
-      ensures materials.plaintextDataKey.Some? ==> res.Success? && materials == res.value
-      ensures res.Success? ==>
-          && materials.encryptionContext == res.value.encryptionContext
-          && materials.algorithmSuiteID == res.value.algorithmSuiteID
-          && (materials.plaintextDataKey.Some? ==> res.value.plaintextDataKey == materials.plaintextDataKey)
-          && materials.verificationKey == res.value.verificationKey
-    {
-      if |edks| == 0 || materials.plaintextDataKey.Some? {
-        return Success(materials);
-      }
-      var i := 0;
-      while i < |edks| {
-        var edk := edks[i];
-        var providerInfo := Failure("Not UTF8");
-        if UTF8.ValidUTF8Seq(edk.providerInfo) && edk.providerID == PROVIDER_ID {
-          providerInfo := UTF8.Decode(edk.providerInfo);
-        }
-        if providerInfo.Success? && ShouldAttemptDecryption(providerInfo.value) {
-          var decryptRequest := KMSUtils.DecryptRequest(edk.ciphertext, materials.encryptionContext, grantTokens);
-          var regionRes := RegionFromKMSKeyARN(providerInfo.value);
-          var regionOpt := regionRes.ToOption();
-          var clientRes := clientSupplier.GetClient(regionOpt);
-          if clientRes.Success? {
-            var client := clientRes.value;
-            var decryptResponseResult := KMSUtils.Decrypt(client, decryptRequest);
-            if decryptResponseResult.Success? {
-              var decryptResponse := decryptResponseResult.value;
-              if (decryptResponse.keyID != providerInfo.value)
-                  || !materials.algorithmSuiteID.ValidPlaintextDataKey(decryptResponse.plaintext) {
-                return Failure("Invalid response from KMS Decrypt");
-              } else {
-                var result := materials.WithPlaintextDataKey(decryptResponse.plaintext);
-                return Success(result);
-              }
-            }
-          }
-        }
-        i := i + 1;
-      }
-      return Success(materials);
-    }
-  }
-}
+//     method OnDecrypt(materials: Mat.ValidDecryptionMaterials, edks: seq<Mat.EncryptedDataKey>) returns (res: Result<Mat.ValidDecryptionMaterials, string>)
+//       requires Valid()
+//       ensures Valid()
+//       ensures |edks| == 0 ==> res.Success? && materials == res.value
+//       ensures materials.plaintextDataKey.Some? ==> res.Success? && materials == res.value
+//       ensures res.Success? ==>
+//           && materials.encryptionContext == res.value.encryptionContext
+//           && materials.algorithmSuiteID == res.value.algorithmSuiteID
+//           && (materials.plaintextDataKey.Some? ==> res.value.plaintextDataKey == materials.plaintextDataKey)
+//           && materials.verificationKey == res.value.verificationKey
+//     {
+//       if |edks| == 0 || materials.plaintextDataKey.Some? {
+//         return Success(materials);
+//       }
+//       var i := 0;
+//       while i < |edks| {
+//         var edk := edks[i];
+//         var providerInfo := Failure("Not UTF8");
+//         if UTF8.ValidUTF8Seq(edk.providerInfo) && edk.providerID == PROVIDER_ID {
+//           providerInfo := UTF8.Decode(edk.providerInfo);
+//         }
+//         if providerInfo.Success? && ShouldAttemptDecryption(providerInfo.value) {
+//           var decryptRequest := KMSUtils.DecryptRequest(edk.ciphertext, materials.encryptionContext, grantTokens);
+//           var regionRes := RegionFromKMSKeyARN(providerInfo.value);
+//           var regionOpt := regionRes.ToOption();
+//           var clientRes := clientSupplier.GetClient(regionOpt);
+//           if clientRes.Success? {
+//             var client := clientRes.value;
+//             var decryptResponseResult := KMSUtils.Decrypt(client, decryptRequest);
+//             if decryptResponseResult.Success? {
+//               var decryptResponse := decryptResponseResult.value;
+//               if (decryptResponse.keyID != providerInfo.value)
+//                   || !materials.algorithmSuiteID.ValidPlaintextDataKey(decryptResponse.plaintext) {
+//                 return Failure("Invalid response from KMS Decrypt");
+//               } else {
+//                 var result := materials.WithPlaintextDataKey(decryptResponse.plaintext);
+//                 return Success(result);
+//               }
+//             }
+//           }
+//         }
+//         i := i + 1;
+//       }
+//       return Success(materials);
+//     }
+//   }
+// }
