src/SDK/Keyring/RawAESKeyring.dfy
@@ -105,12 +105,7 @@ module {:extern "RawAESKeyringDef"} RawAESKeyringDef {
     method OnEncrypt(materials: Mat.ValidEncryptionMaterials) returns (res: Result<Mat.ValidEncryptionMaterials, string>)
       // Keyring Trait conditions
       requires Valid()
-      ensures res.Success? ==>
-        && materials.encryptionContext == res.value.encryptionContext
-        && materials.algorithmSuiteID == res.value.algorithmSuiteID
-        && (materials.plaintextDataKey.Some? ==> res.value.plaintextDataKey == materials.plaintextDataKey)
-        && materials.encryptedDataKeys <= res.value.encryptedDataKeys
-        && materials.signingKey == res.value.signingKey
+      ensures KeyringDefs.OnEncryptPure(materials, res)
 
       // EDK created using expected AAD
       ensures res.Success? ==>
@@ -170,13 +165,7 @@ module {:extern "RawAESKeyringDef"} RawAESKeyringDef {
       // Keyring Trait conditions
       requires Valid()
       ensures Valid()
-      ensures |edks| == 0 ==> res.Success? && materials == res.value
-      ensures materials.plaintextDataKey.Some? ==> res.Success? && materials == res.value
-      ensures res.Success? ==>
-          && materials.encryptionContext == res.value.encryptionContext
-          && materials.algorithmSuiteID == res.value.algorithmSuiteID
-          && (materials.plaintextDataKey.Some? ==> res.value.plaintextDataKey == materials.plaintextDataKey)
-          && res.value.verificationKey == materials.verificationKey
+      ensures KeyringDefs.OnDecryptPure(materials, res)
 
       // TODO: ensure non-None when input edk list has edk with valid provider info
 
@@ -220,7 +209,7 @@ module {:extern "RawAESKeyringDef"} RawAESKeyringDef {
         }
         i := i + 1;
       }
-      return Success(materials);
+      return Failure("Unable to decrypt.");
     }
 
     predicate method ShouldDecryptEDK(edk: Mat.EncryptedDataKey) {
