src/StandardLibrary/Actions.dfy
@@ -1,0 +1,167 @@
+// Copyright Amazon.com Inc. or its affiliates. All Rights Reserved.
+// SPDX-License-Identifier: Apache-2.0
+
+include "../../libraries/src/Wrappers.dfy"
+
+module Actions {
+
+  import opened Wrappers
+
+  trait {:termination false} Action<A, R>
+  {
+    method Invoke(a: A)
+      returns (r: R)
+      ensures Ensures(a, r)
+    predicate Ensures(a: A, r: R)
+  }
+
+  trait {:termination false} ActionWithResult<A, R, E>
+    extends Action<A, Result<R, E>>
+  {
+    method Invoke(a: A)
+      returns (res: Result<R, E>)
+      ensures Ensures(a, res)
+  }
+
+  method Map<A, R>(
+    action: Action<A, R>,
+    s: seq<A>
+  )
+    returns (res: seq<R>)
+    ensures |s| == |res|
+    ensures
+      forall i ::
+        && 0 <= i < |s|
+      ==>
+        action.Ensures(s[i], res[i])
+  {
+    var rs := [];
+    for i := 0 to |s|
+      invariant |s[..i]| == |rs|
+      invariant forall j ::
+        && 0 <= j < i
+      ==>
+        action.Ensures(s[j], rs[j])
+    {
+      var r := action.Invoke(s[i]);
+      rs := rs + [r];
+    }
+    return rs;
+  }
+
+  method MapWithResult<A, R, E>(
+    action: ActionWithResult<A, R, E>,
+    s: seq<A>
+  )
+    returns (res: Result<seq<R>, E>)
+    ensures
+      res.Success?
+    ==>
+      |s| == |res.value|
+    ensures
+      res.Success?
+    ==>
+        (forall i ::
+          && 0 <= i < |s|
+        ==>
+          action.Ensures(s[i], Success(res.value[i])))
+  {
+    var rs := [];
+    for i := 0 to |s|
+      invariant |s[..i]| == |rs|
+      invariant forall j ::
+        && 0 <= j < i
+      ==>
+        action.Ensures(s[j], Success(rs[j]))
+    {
+      var r :- action.Invoke(s[i]);
+      rs := rs + [r];
+    }
+    return Success(rs);
+  }
+
+  method Filter<A>(
+    action: Action<A, bool>,
+    s: seq<A>
+  )
+    returns (res: seq<A>)
+    ensures |s| >= |res|
+    ensures
+      forall j ::
+        j in res
+      ==>
+        && j in s
+        && action.Ensures(j, true)
+  {
+    var rs := [];
+    for i := 0 to |s|
+      invariant |s[..i]| >= |rs|
+      invariant forall j ::
+        j in rs
+      ==>
+        && j in s
+        && action.Ensures(j, true)
+    {
+      var r := action.Invoke(s[i]);
+      if r {
+        rs := rs + [s[i]];
+      }
+    }
+    return rs;
+  }
+
+
+  method FilterWithResult<A, E>(
+    action: ActionWithResult<A, bool, E>,
+    s: seq<A>
+  )
+    returns (res: Result<seq<A>, E>)
+    ensures
+      res.Success?
+    ==>
+      && |s| >= |res.value|
+      && forall j ::
+        j in res.value
+      ==>
+        && j in s
+        && action.Ensures(j, Success(true))
+  {
+    var rs := [];
+    for i := 0 to |s|
+      invariant |s[..i]| >= |rs|
+      invariant forall j ::
+        j in rs
+      ==>
+        && j in s
+        && action.Ensures(j, Success(true))
+    {
+      var r :- action.Invoke(s[i]);
+      if r {
+        rs := rs + [s[i]];
+      }
+    }
+    return Success(rs);
+  }
+
+  method ReduceToSuccess<A, B, E>(
+    action: ActionWithResult<A, B, E>,
+    s: seq<A>
+  )
+    returns (res: Result<B, seq<E>>)
+    ensures
+      res.Success?
+    ==>
+      exists a | a in s :: action.Ensures(a, Success(res.value))
+  {
+    var errors := [];
+    for i := 0 to |s| {
+      var attempt := action.Invoke(s[i]);
+      if attempt.Success? {
+        return Success(attempt.value);
+      } else {
+        errors := errors + [attempt.error];
+      }
+    }
+    return Failure(errors);
+  }
+}
